src/Boolify/src/DecodeScript.sml
@@ -3,12 +3,13 @@
 (*===========================================================================*)
 
 (* Interactive mode
-app load ["bossLib", "rich_listTheory", "EncodeTheory", "normalForms"];
+app load
+["bossLib", "rich_listTheory", "EncodeTheory", "normalForms", "metisLib"];
 *)
 
 open HolKernel boolLib Parse bossLib pairTheory pairTools
      arithmeticTheory listTheory rich_listTheory EncodeTheory
-     mesonLib optionTheory normalForms combinTheory;
+     metisLib optionTheory normalForms combinTheory;
 
 val _ = new_theory "Decode";
 
@@ -24,18 +25,6 @@ val Suff = Q_TAC SUFF_TAC;
 val Know = Q_TAC KNOW_TAC;
 
 val REVERSE = Tactical.REVERSE;
-
-(*---------------------------------------------------------------------------
-     decode turns a decoding parser of type
-
-       bool list -> ('a # bool list) option
-
-     into a straight function of type
-
-       bool list -> 'a
- ---------------------------------------------------------------------------*)
-
-val decode_def = Define `decode f = FST o THE o f`;
 
 (*---------------------------------------------------------------------------
      Well-formed decoders: the definition is carefully chosen to be the
@@ -97,6 +86,17 @@ val enc2dec_some = store_thm
    Suff `q = x` >> PROVE_TAC [APPEND_11] ++
    FULL_SIMP_TAC std_ss [wf_encoder_def] ++
    PROVE_TAC [IS_PREFIX_APPEND1, IS_PREFIX_APPEND2, IS_PREFIX_REFL]);
+
+val enc2dec_some_alt = store_thm
+  ("enc2dec_some_alt",
+   ``!p e l x.
+       wf_encoder p e ==>
+       ((enc2dec p e l = SOME x) =
+        p (FST x) /\ (l = APPEND (e (FST x)) (SND x)))``,
+   RW_TAC std_ss []
+   ++ Cases_on `x`
+   ++ RW_TAC std_ss [FST, SND]
+   ++ HO_METIS_TAC [enc2dec_some]);
 
 val wf_enc2dec = store_thm
   ("wf_enc2dec",
@@ -206,64 +206,410 @@ val enc2dec_dec2enc = store_thm
     RW_TAC std_ss [APPEND_NIL]]);
 
 (*---------------------------------------------------------------------------
+     Unit decoders
+ ---------------------------------------------------------------------------*)
+
+val decode_unit_def = Define `decode_unit p = enc2dec p encode_unit`;
+
+val wf_decode_unit = store_thm
+  ("wf_decode_unit",
+   ``wf_decoder p (decode_unit p)``,
+   RW_TAC std_ss [decode_unit_def, wf_enc2dec, wf_encode_unit]);
+
+val dec2enc_decode_unit = store_thm
+  ("dec2enc_decode_unit",
+   ``!p x. p x ==> (dec2enc (decode_unit p) x = encode_unit x)``,
+   RW_TAC std_ss [decode_unit_def, dec2enc_enc2dec, wf_encode_unit]);
+
+val decode_unit = store_thm
+  ("decode_unit",
+   ``decode_unit p l = if p () then SOME ((), l) else NONE``,
+   RW_TAC std_ss
+   [decode_unit_def, enc2dec_none, enc2dec_some, encode_unit_def,
+    APPEND, wf_encode_unit, oneTheory.one]);
+
+(*---------------------------------------------------------------------------
      Boolean decoders
  ---------------------------------------------------------------------------*)
 
-val dec_bool_def = Define `dec_bool = enc2dec total encode_bool`;
+val decode_bool_def = Define `decode_bool p = enc2dec p encode_bool`;
 
-val decode_bool_def = Define `decode_bool = decode dec_bool`;
+val wf_decode_bool = store_thm
+  ("wf_decode_bool",
+   ``!p. wf_decoder p (decode_bool p)``,
+   RW_TAC std_ss [decode_bool_def, wf_enc2dec, wf_encode_bool]);
 
-val wf_dec_bool = store_thm
-  ("wf_dec_bool",
-   ``wf_decoder total dec_bool``,
-   RW_TAC std_ss [dec_bool_def, wf_enc2dec, wf_encode_bool]);
+val dec2enc_decode_bool = store_thm
+  ("dec2enc_decode_bool",
+   ``!p x. p x ==> (dec2enc (decode_bool p) x = encode_bool x)``,
+   RW_TAC std_ss [decode_bool_def, dec2enc_enc2dec, wf_encode_bool]);
 
-val dec2enc_dec_bool = store_thm
-  ("dec2enc_dec_bool",
-   ``dec2enc dec_bool = encode_bool``,
-   MATCH_MP_TAC EQ_EXT ++
-   RW_TAC std_ss
-   [dec_bool_def, dec2enc_enc2dec, wf_encode_bool, total_def]);
-
-val dec_bool = store_thm
-  ("dec_bool",
-   ``dec_bool l = case l of [] -> NONE || (h :: t) -> SOME (h, t)``,
+val decode_bool = store_thm
+  ("decode_bool",
+   ``decode_bool p l =
+     case l of [] -> NONE || (h :: t) -> if p h then SOME (h, t) else NONE``,
    REPEAT CASE_TAC ++
    RW_TAC std_ss
-   [dec_bool_def, enc2dec_none, enc2dec_some, encode_bool_def,
-    APPEND, wf_encode_bool, total_def]);
+   [decode_bool_def, enc2dec_none, enc2dec_some, encode_bool_def,
+    APPEND, wf_encode_bool]);
+
+(*---------------------------------------------------------------------------
+     Pair decoders
+ ---------------------------------------------------------------------------*)
+
+val decode_prod_def = Define
+  `decode_prod p d1 d2 = enc2dec p (encode_prod (dec2enc d1) (dec2enc d2))`;
+
+val wf_decode_prod = store_thm
+  ("wf_decode_prod",
+   ``!p1 p2 d1 d2.
+       wf_decoder p1 d1 /\ wf_decoder p2 d2 ==>
+       wf_decoder (lift_prod p1 p2) (decode_prod (lift_prod p1 p2) d1 d2)``,
+   RW_TAC std_ss [decode_prod_def] ++
+   PROVE_TAC [wf_dec2enc, wf_enc2dec, wf_encode_prod]);
+
+val dec2enc_decode_prod = store_thm
+  ("dec2enc_decode_prod",
+   ``!p1 p2 d1 d2 x.
+       wf_decoder p1 d1 /\ wf_decoder p2 d2 /\ lift_prod p1 p2 x ==>
+       (dec2enc (decode_prod (lift_prod p1 p2) d1 d2) x =
+        encode_prod (dec2enc d1) (dec2enc d2) x)``,
+   RW_TAC std_ss
+   [decode_prod_def, dec2enc_enc2dec, wf_encode_prod, wf_dec2enc]);
+
+val encode_then_decode_prod = store_thm
+  ("decode_encode_prod",
+   ``!p1 p2 e1 e2 l t.
+       wf_encoder p1 e1 /\ wf_encoder p2 e2 /\ lift_prod p1 p2 l ==>
+       (decode_prod (lift_prod p1 p2) (enc2dec p1 e1) (enc2dec p2 e2)
+        (APPEND (encode_prod e1 e2 l) t) = SOME (l, t))``,
+   RW_TAC std_ss [decode_prod_def] ++
+   MP_TAC
+   (Q.SPECL
+    [`lift_prod p1 p2`,
+     `encode_prod (dec2enc (enc2dec p1 e1)) (dec2enc (enc2dec p2 e2))`,
+     `APPEND (encode_prod e1 e2 l) t`, `l`, `t`]
+    (INST_TYPE [alpha |-> ``:'a # 'b``] enc2dec_some)) ++
+   MATCH_MP_TAC (PROVE [] ``x /\ (y ==> z) ==> (x ==> y) ==> z``) ++
+   CONJ_TAC >> PROVE_TAC [wf_encode_prod, wf_dec2enc, wf_enc2dec] ++
+   RW_TAC std_ss [APPEND_11] ++
+   POP_ASSUM (K ALL_TAC) ++
+   Cases_on `l` ++
+   FULL_SIMP_TAC std_ss [lift_prod_def, encode_prod_def, APPEND_11] ++
+   PROVE_TAC [dec2enc_enc2dec]);
+
+val decode_prod = store_thm
+  ("decode_prod",
+   ``wf_decoder p1 d1 /\ wf_decoder p2 d2 ==>
+     (decode_prod (lift_prod p1 p2) d1 d2 l =
+      case d1 l of NONE -> NONE
+      || SOME (x, t) ->
+         (case d2 t of NONE -> NONE
+          || SOME (y, t') -> SOME ((x, y), t')))``,
+   (REPEAT CASE_TAC ++
+    RW_TAC std_ss
+    [decode_prod_def, enc2dec_none, GSYM APPEND_ASSOC, encode_prod_alt]) <<
+   [STRIP_TAC
+    ++ RW_TAC std_ss []
+    ++ Cases_on `x`
+    ++ FULL_SIMP_TAC std_ss [lift_prod_def]
+    ++ PROVE_TAC [decode_dec2enc_append, NOT_SOME_NONE],
+    STRIP_TAC
+    ++ RW_TAC std_ss []
+    ++ Cases_on `x`
+    ++ FULL_SIMP_TAC std_ss [lift_prod_def]
+    ++ Q.PAT_ASSUM `X = SOME Y` MP_TAC
+    ++ MP_TAC (Q.SPECL [`p1`, `d1`, `q'`] decode_dec2enc_append)
+    ++ ASM_SIMP_TAC std_ss []
+    ++ DISCH_THEN (K ALL_TAC)
+    ++ PURE_REWRITE_TAC [GSYM DE_MORGAN_THM]
+    ++ STRIP_TAC
+    ++ RW_TAC std_ss []
+    ++ Q.PAT_ASSUM `X = Y` MP_TAC
+    ++ RW_TAC std_ss [decode_prod_def, enc2dec_none]
+    ++ PROVE_TAC [decode_dec2enc_append, NOT_SOME_NONE],
+    Know `wf_decoder (lift_prod p1 p2) (decode_prod (lift_prod p1 p2) d1 d2)`
+    >> PROVE_TAC [wf_decode_prod]
+    ++ STRIP_TAC
+    ++ Know `wf_encoder p1 (dec2enc d1)` >> PROVE_TAC [wf_dec2enc]
+    ++ STRIP_TAC
+    ++ Know `wf_encoder p2 (dec2enc d2)` >> PROVE_TAC [wf_dec2enc]
+    ++ STRIP_TAC
+    ++ Know
+       `wf_encoder (lift_prod p1 p2) (encode_prod (dec2enc d1) (dec2enc d2))`
+    >> PROVE_TAC [wf_encode_prod]
+    ++ STRIP_TAC
+    ++ ASM_SIMP_TAC std_ss [enc2dec_some, encode_prod_def, APPEND]
+    ++ MATCH_MP_TAC (PROVE [] ``x /\ (x ==> y) ==> x /\ y``)
+    ++ CONJ_TAC
+    >> (RW_TAC std_ss [lift_prod_def]
+        ++ PROVE_TAC [wf_decoder_def, wf_decode_prod])
+    ++ RW_TAC std_ss [lift_prod_def]
+    ++ MP_TAC (Q.SPECL [`p1`, `d1`] wf_decoder_def)
+    ++ ASM_SIMP_TAC std_ss []
+    ++ DISCH_THEN (MP_TAC o Q.SPEC `q`)
+    ++ RW_TAC std_ss []
+    ++ RES_TAC
+    ++ RW_TAC std_ss [GSYM APPEND_ASSOC]
+    ++ Know `dec2enc d1 q = a` >> PROVE_TAC [APPEND_NIL, dec2enc_some]
+    ++ RW_TAC std_ss [APPEND_11]
+    ++ Q.PAT_ASSUM `!x. P x` (K ALL_TAC)
+    ++ MP_TAC (Q.SPECL [`p2`, `d2`] (INST_TYPE [alpha |-> beta] wf_decoder_def))
+    ++ ASM_SIMP_TAC std_ss []
+    ++ DISCH_THEN (MP_TAC o Q.SPEC `q'`)
+    ++ RW_TAC std_ss []
+    ++ RES_TAC
+    ++ RW_TAC std_ss [GSYM APPEND_ASSOC]
+    ++ Know `dec2enc d2 q' = a` >> PROVE_TAC [APPEND_NIL, dec2enc_some]
+    ++ RW_TAC std_ss [APPEND_11]]);
+
+(*---------------------------------------------------------------------------
+     Sum decoders
+ ---------------------------------------------------------------------------*)
+
+val decode_sum_def = Define
+  `decode_sum p d1 d2 = enc2dec p (encode_sum (dec2enc d1) (dec2enc d2))`;
+
+val wf_decode_sum = store_thm
+  ("wf_decode_sum",
+   ``!p1 p2 d1 d2.
+       wf_decoder p1 d1 /\ wf_decoder p2 d2 ==>
+       wf_decoder (lift_sum p1 p2) (decode_sum (lift_sum p1 p2) d1 d2)``,
+   RW_TAC std_ss [decode_sum_def] ++
+   PROVE_TAC [wf_dec2enc, wf_enc2dec, wf_encode_sum]);
+
+val dec2enc_decode_sum = store_thm
+  ("dec2enc_decode_sum",
+   ``!p1 p2 d1 d2 x.
+       wf_decoder p1 d1 /\ wf_decoder p2 d2 /\ lift_sum p1 p2 x ==>
+       (dec2enc (decode_sum (lift_sum p1 p2) d1 d2) x =
+        encode_sum (dec2enc d1) (dec2enc d2) x)``,
+   RW_TAC std_ss
+   [decode_sum_def, dec2enc_enc2dec, wf_encode_sum, wf_dec2enc]);
+
+val encode_then_decode_sum = store_thm
+  ("decode_encode_sum",
+   ``!p1 p2 e1 e2 l t.
+       wf_encoder p1 e1 /\ wf_encoder p2 e2 /\ lift_sum p1 p2 l ==>
+       (decode_sum (lift_sum p1 p2) (enc2dec p1 e1) (enc2dec p2 e2)
+        (APPEND (encode_sum e1 e2 l) t) = SOME (l, t))``,
+   RW_TAC std_ss [decode_sum_def] ++
+   MP_TAC
+   (Q.SPECL
+    [`lift_sum p1 p2`,
+     `encode_sum (dec2enc (enc2dec p1 e1)) (dec2enc (enc2dec p2 e2))`,
+     `APPEND (encode_sum e1 e2 l) t`, `l`, `t`]
+    (INST_TYPE [alpha |-> ``:'a + 'b``] enc2dec_some)) ++
+   MATCH_MP_TAC (PROVE [] ``x /\ (y ==> z) ==> (x ==> y) ==> z``) ++
+   CONJ_TAC >> PROVE_TAC [wf_encode_sum, wf_dec2enc, wf_enc2dec] ++
+   RW_TAC std_ss [APPEND_11] ++
+   POP_ASSUM (K ALL_TAC) ++
+   Cases_on `l` ++
+   FULL_SIMP_TAC std_ss [lift_sum_def, encode_sum_def, APPEND_11] ++
+   PROVE_TAC [dec2enc_enc2dec]);
+
+val decode_sum = store_thm
+  ("decode_sum",
+   ``wf_decoder p1 d1 /\ wf_decoder p2 d2 ==>
+     (decode_sum (lift_sum p1 p2) d1 d2 l =
+      case l of [] -> NONE
+      || (T :: t) ->
+         (case d1 t of NONE -> NONE
+          || SOME (x, t') -> SOME (INL x, t'))
+      || (F :: t) ->
+         (case d2 t of NONE -> NONE
+          || SOME (x, t') -> SOME (INR x, t')))``,
+   (REPEAT CASE_TAC ++
+    RW_TAC std_ss [decode_sum_def, enc2dec_none, GSYM APPEND_ASSOC]) <<
+   [Cases_on `x`
+    ++ RW_TAC std_ss [encode_sum_def, APPEND],
+    (Cases_on `x` ++ RW_TAC std_ss [encode_sum_def, APPEND])
+    ++ STRIP_TAC
+    ++ RW_TAC std_ss []
+    ++ FULL_SIMP_TAC std_ss [lift_sum_def]
+    ++ PROVE_TAC [decode_dec2enc_append, NOT_SOME_NONE],
+    Know `wf_decoder (lift_sum p1 p2) (decode_sum (lift_sum p1 p2) d1 d2)`
+    >> PROVE_TAC [wf_decode_sum]
+    ++ STRIP_TAC
+    ++ Know `wf_encoder p1 (dec2enc d1)` >> PROVE_TAC [wf_dec2enc]
+    ++ STRIP_TAC
+    ++ Know `wf_encoder p2 (dec2enc d2)` >> PROVE_TAC [wf_dec2enc]
+    ++ STRIP_TAC
+    ++ Know
+       `wf_encoder (lift_sum p1 p2) (encode_sum (dec2enc d1) (dec2enc d2))`
+    >> PROVE_TAC [wf_encode_sum]
+    ++ STRIP_TAC
+    ++ ASM_SIMP_TAC std_ss [enc2dec_some, encode_sum_def, APPEND]
+    ++ MATCH_MP_TAC (PROVE [] ``x /\ (x ==> y) ==> x /\ y``)
+    ++ CONJ_TAC
+    >> (RW_TAC std_ss [lift_sum_def]
+        ++ PROVE_TAC [wf_decoder_def, wf_decode_sum])
+    ++ RW_TAC std_ss [lift_sum_def]
+    ++ MP_TAC (Q.SPECL [`p1`, `d1`] wf_decoder_def)
+    ++ ASM_SIMP_TAC std_ss []
+    ++ DISCH_THEN (MP_TAC o Q.SPEC `q`)
+    ++ RW_TAC std_ss []
+    ++ RES_TAC
+    ++ RW_TAC std_ss [GSYM APPEND_ASSOC]
+    ++ Know `dec2enc d1 q = a` >> PROVE_TAC [APPEND_NIL, dec2enc_some]
+    ++ RW_TAC std_ss [APPEND_11],
+    (Cases_on `x` ++ RW_TAC std_ss [encode_sum_def, APPEND])
+    ++ STRIP_TAC
+    ++ RW_TAC std_ss []
+    ++ FULL_SIMP_TAC std_ss [lift_sum_def]
+    ++ PROVE_TAC [decode_dec2enc_append, NOT_SOME_NONE],
+    Know `wf_decoder (lift_sum p1 p2) (decode_sum (lift_sum p1 p2) d1 d2)`
+    >> PROVE_TAC [wf_decode_sum]
+    ++ STRIP_TAC
+    ++ Know `wf_encoder p1 (dec2enc d1)` >> PROVE_TAC [wf_dec2enc]
+    ++ STRIP_TAC
+    ++ Know `wf_encoder p2 (dec2enc d2)` >> PROVE_TAC [wf_dec2enc]
+    ++ STRIP_TAC
+    ++ Know
+       `wf_encoder (lift_sum p1 p2) (encode_sum (dec2enc d1) (dec2enc d2))`
+    >> PROVE_TAC [wf_encode_sum]
+    ++ STRIP_TAC
+    ++ ASM_SIMP_TAC std_ss [enc2dec_some, encode_sum_def, APPEND]
+    ++ MATCH_MP_TAC (PROVE [] ``x /\ (x ==> y) ==> x /\ y``)
+    ++ CONJ_TAC
+    >> (RW_TAC std_ss [lift_sum_def]
+        ++ PROVE_TAC [wf_decoder_def, wf_decode_sum])
+    ++ RW_TAC std_ss [lift_sum_def]
+    ++ MP_TAC (Q.SPECL [`p2`, `d2`] wf_decoder_def)
+    ++ ASM_SIMP_TAC std_ss []
+    ++ DISCH_THEN (MP_TAC o Q.SPEC `q`)
+    ++ RW_TAC std_ss []
+    ++ RES_TAC
+    ++ RW_TAC std_ss [GSYM APPEND_ASSOC]
+    ++ Know `dec2enc d2 q = a` >> PROVE_TAC [APPEND_NIL, dec2enc_some]
+    ++ RW_TAC std_ss [APPEND_11]]);
+
+(*---------------------------------------------------------------------------
+     Option decoders
+ ---------------------------------------------------------------------------*)
+
+val decode_option_def = Define
+  `decode_option p d = enc2dec p (encode_option (dec2enc d))`;
+
+val wf_decode_option = store_thm
+  ("wf_decode_option",
+   ``!p d.
+       wf_decoder p d ==>
+       wf_decoder (lift_option p) (decode_option (lift_option p) d)``,
+   RW_TAC std_ss [decode_option_def] ++
+   PROVE_TAC [wf_dec2enc, wf_enc2dec, wf_encode_option]);
+
+val dec2enc_decode_option = store_thm
+  ("dec2enc_decode_option",
+   ``!p d x.
+       wf_decoder p d /\ lift_option p x ==>
+       (dec2enc (decode_option (lift_option p) d) x =
+        encode_option (dec2enc d) x)``,
+   RW_TAC std_ss
+   [decode_option_def, dec2enc_enc2dec, wf_encode_option, wf_dec2enc]);
+
+val encode_then_decode_option = store_thm
+  ("decode_encode_option",
+   ``!p e l t.
+       wf_encoder p e /\ lift_option p l ==>
+       (decode_option (lift_option p) (enc2dec p e)
+        (APPEND (encode_option e l) t) = SOME (l, t))``,
+   RW_TAC std_ss [decode_option_def] ++
+   MP_TAC
+   (Q.SPECL [`lift_option p`, `encode_option (dec2enc (enc2dec p e))`,
+             `APPEND (encode_option e l) t`, `l`, `t`]
+    (INST_TYPE [alpha |-> ``:'a option``] enc2dec_some)) ++
+   MATCH_MP_TAC (PROVE [] ``x /\ (y ==> z) ==> (x ==> y) ==> z``) ++
+   CONJ_TAC >> PROVE_TAC [wf_encode_option, wf_dec2enc, wf_enc2dec] ++
+   RW_TAC std_ss [APPEND_11] ++
+   POP_ASSUM (K ALL_TAC) ++
+   Cases_on `l` ++
+   FULL_SIMP_TAC std_ss [lift_option_def, encode_option_def, APPEND_11] ++
+   RW_TAC std_ss [] ++
+   PROVE_TAC [dec2enc_enc2dec]);
+
+val decode_option = store_thm
+  ("decode_option",
+   ``wf_decoder p d ==>
+     (decode_option (lift_option p) d l =
+      case l of [] -> NONE
+      || (T :: t) ->
+         (case d t of NONE -> NONE
+          || SOME (x, t') -> SOME (SOME x, t'))
+      || (F :: t) -> SOME (NONE, t))``,
+   (REPEAT CASE_TAC ++
+    RW_TAC std_ss [decode_option_def, enc2dec_none]) <<
+   [Cases_on `x`
+    ++ RW_TAC std_ss [encode_option_def, APPEND],
+    Cases_on `x`
+    ++ POP_ASSUM MP_TAC
+    ++ RW_TAC std_ss
+       [encode_option_def, APPEND, GSYM APPEND_ASSOC, lift_option_def]
+    ++ STRIP_TAC
+    ++ RW_TAC std_ss []
+    ++ MP_TAC (Q.SPECL [`p`, `d`] wf_decoder_def)
+    ++ RW_TAC std_ss []
+    ++ Q.EXISTS_TAC `x'`
+    ++ RW_TAC std_ss []
+    ++ PROVE_TAC [decode_dec2enc_append, NOT_SOME_NONE],
+    Know `wf_decoder (lift_option p) (decode_option (lift_option p) d)`
+    >> PROVE_TAC [wf_decode_option]
+    ++ STRIP_TAC
+    ++ Know `wf_encoder p (dec2enc d)` >> PROVE_TAC [wf_dec2enc]
+    ++ STRIP_TAC
+    ++ Know `wf_encoder (lift_option p) (encode_option (dec2enc d))`
+    >> PROVE_TAC [wf_encode_option]
+    ++ STRIP_TAC
+    ++ ASM_SIMP_TAC std_ss
+       [enc2dec_some, encode_option_def, APPEND, lift_option_def]
+    ++ MATCH_MP_TAC (PROVE [] ``x /\ (x ==> y) ==> x /\ y``)
+    ++ CONJ_TAC >> PROVE_TAC [wf_decoder_def, wf_decode_option]
+    ++ RW_TAC std_ss []
+    ++ MP_TAC (Q.SPECL [`p`, `d`] wf_decoder_def)
+    ++ ASM_SIMP_TAC std_ss []
+    ++ DISCH_THEN (MP_TAC o Q.SPEC `q`)
+    ++ RW_TAC std_ss []
+    ++ RES_TAC
+    ++ RW_TAC std_ss [GSYM APPEND_ASSOC]
+    ++ Know `dec2enc d q = a` >> PROVE_TAC [APPEND_NIL, dec2enc_some]
+    ++ RW_TAC std_ss [APPEND_11],
+    Know `wf_encoder p (dec2enc d)` >> PROVE_TAC [wf_dec2enc]
+    ++ STRIP_TAC
+    ++ Know `wf_encoder (lift_option p) (encode_option (dec2enc d))`
+    >> PROVE_TAC [wf_encode_option]
+    ++ STRIP_TAC
+    ++ ASM_SIMP_TAC std_ss
+       [enc2dec_some, encode_option_def, APPEND, lift_option_def]]);
 
 (*---------------------------------------------------------------------------
      List decoders
  ---------------------------------------------------------------------------*)
 
-val dec_list_def = Define
-  `dec_list p d = enc2dec p (encode_list (dec2enc d))`;
+val decode_list_def = Define
+  `decode_list p d = enc2dec p (encode_list (dec2enc d))`;
 
-val decode_list_def = Define `decode_list p d = decode (dec_list p d)`;
-
-val wf_dec_list = store_thm
-  ("wf_dec_list",
+val wf_decode_list = store_thm
+  ("wf_decode_list",
    ``!p d.
-       wf_decoder p d ==> wf_decoder (EVERY p) (dec_list (EVERY p) d)``,
-   RW_TAC std_ss [dec_list_def] ++
+       wf_decoder p d ==> wf_decoder (EVERY p) (decode_list (EVERY p) d)``,
+   RW_TAC std_ss [decode_list_def] ++
    PROVE_TAC [wf_dec2enc, wf_enc2dec, wf_encode_list]);
 
-val dec2enc_dec_list = store_thm
-  ("dec2enc_dec_list",
+val dec2enc_decode_list = store_thm
+  ("dec2enc_decode_list",
    ``!p d x.
        wf_decoder p d /\ EVERY p x ==>
-       (dec2enc (dec_list (EVERY p) d) x = encode_list (dec2enc d) x)``,
+       (dec2enc (decode_list (EVERY p) d) x = encode_list (dec2enc d) x)``,
    RW_TAC std_ss
-   [dec_list_def, dec2enc_enc2dec, wf_encode_list, wf_dec2enc]);
+   [decode_list_def, dec2enc_enc2dec, wf_encode_list, wf_dec2enc]);
 
-val encode_then_dec_list = store_thm
+val encode_then_decode_list = store_thm
   ("decode_encode_list",
    ``!p e l t.
        wf_encoder p e /\ EVERY p l ==>
-       (dec_list (EVERY p) (enc2dec p e) (APPEND (encode_list e l) t) =
+       (decode_list (EVERY p) (enc2dec p e) (APPEND (encode_list e l) t) =
         SOME (l, t))``,
-   RW_TAC std_ss [dec_list_def] ++
+   RW_TAC std_ss [decode_list_def] ++
    MP_TAC
    (Q.SPECL [`EVERY p`, `encode_list (dec2enc (enc2dec p e))`,
              `APPEND (encode_list e l) t`, `l`, `t`]
@@ -276,19 +622,19 @@ val encode_then_dec_list = store_thm
    RW_TAC std_ss [EVERY_DEF, encode_list_def, APPEND_11] ++
    PROVE_TAC [dec2enc_enc2dec]);
 
-val dec_list = store_thm
-  ("dec_list",
+val decode_list = store_thm
+  ("decode_list",
    ``wf_decoder p d ==>
-     (dec_list (EVERY p) d l =
+     (decode_list (EVERY p) d l =
       case l of [] -> NONE
       || (T :: t) ->
          (case d t of NONE -> NONE
           || SOME (x, t') ->
-             (case dec_list (EVERY p) d t' of NONE -> NONE
+             (case decode_list (EVERY p) d t' of NONE -> NONE
               || SOME (xs, t'') -> SOME (x :: xs, t'')))
       || (F :: t) -> SOME ([], t))``,
    (REPEAT CASE_TAC ++
-    RW_TAC std_ss [dec_list_def, enc2dec_none]) <<
+    RW_TAC std_ss [decode_list_def, enc2dec_none]) <<
    [Cases_on `x` ++
     RW_TAC std_ss [encode_list_def, APPEND],
     Cases_on `x` ++
@@ -316,10 +662,10 @@ val dec_list = store_thm
     STRIP_TAC ++
     RW_TAC std_ss [] ++
     Q.PAT_ASSUM `X = Y` MP_TAC ++
-    RW_TAC std_ss [dec_list_def, enc2dec_none] ++
+    RW_TAC std_ss [decode_list_def, enc2dec_none] ++
     PROVE_TAC [],
-    Know `wf_decoder (EVERY p) (dec_list (EVERY p) d)` >>
-    PROVE_TAC [wf_dec_list] ++
+    Know `wf_decoder (EVERY p) (decode_list (EVERY p) d)` >>
+    PROVE_TAC [wf_decode_list] ++
     STRIP_TAC ++
     Know `wf_encoder p (dec2enc d)` >> PROVE_TAC [wf_dec2enc] ++
     STRIP_TAC ++
@@ -328,7 +674,7 @@ val dec_list = store_thm
     STRIP_TAC ++
     ASM_SIMP_TAC std_ss [enc2dec_some, encode_list_def, APPEND] ++
     MATCH_MP_TAC (PROVE [] ``x /\ (x ==> y) ==> x /\ y``) ++
-    CONJ_TAC >> PROVE_TAC [EVERY_DEF, wf_decoder_def, wf_dec_list] ++
+    CONJ_TAC >> PROVE_TAC [EVERY_DEF, wf_decoder_def, wf_decode_list] ++
     RW_TAC std_ss [EVERY_DEF] ++
     MP_TAC (Q.SPECL [`p`, `d`] wf_decoder_def) ++
     ASM_SIMP_TAC std_ss [] ++
@@ -340,7 +686,7 @@ val dec_list = store_thm
     RW_TAC std_ss [APPEND_11] ++
     Q.PAT_ASSUM `!x. P x` (K ALL_TAC) ++
     MP_TAC
-    (Q.ISPECL [`EVERY (p : 'a -> bool)`, `dec_list (EVERY p) d`]
+    (Q.ISPECL [`EVERY (p : 'a -> bool)`, `decode_list (EVERY p) d`]
      wf_decoder_def) ++
     ASM_SIMP_TAC std_ss [] ++
     DISCH_THEN (MP_TAC o Q.SPEC `q'`) ++
@@ -349,9 +695,9 @@ val dec_list = store_thm
     RW_TAC std_ss [] ++
     Q.PAT_ASSUM `!x. P x` (K ALL_TAC) ++
     Q.PAT_ASSUM `X = Y` MP_TAC ++
-    ASM_SIMP_TAC std_ss [dec_list_def, enc2dec_some],
-    Know `wf_decoder (EVERY p) (dec_list (EVERY p) d)` >>
-    PROVE_TAC [wf_dec_list] ++
+    ASM_SIMP_TAC std_ss [decode_list_def, enc2dec_some],
+    Know `wf_decoder (EVERY p) (decode_list (EVERY p) d)` >>
+    PROVE_TAC [wf_decode_list] ++
     STRIP_TAC ++
     Know `wf_encoder p (dec2enc d)` >> PROVE_TAC [wf_dec2enc] ++
     STRIP_TAC ++
@@ -361,42 +707,162 @@ val dec_list = store_thm
     ASM_SIMP_TAC std_ss [enc2dec_some, encode_list_def, APPEND, EVERY_DEF]]);
 
 (*---------------------------------------------------------------------------
+     Num decoders
+ ---------------------------------------------------------------------------*)
+
+val decode_num_def = Define `decode_num p = enc2dec p encode_num`;
+
+val wf_decode_num = store_thm
+  ("wf_decode_num",
+   ``!p. wf_decoder p (decode_num p)``,
+   RW_TAC std_ss [decode_num_def, wf_enc2dec, wf_encode_num]);
+
+val dec2enc_decode_num = store_thm
+  ("dec2enc_decode_num",
+   ``!p x. p x ==> (dec2enc (decode_num p) x = encode_num x)``,
+   RW_TAC std_ss [decode_num_def, dec2enc_enc2dec, wf_encode_num]);
+
+(*
+val decode_num = store_thm
+  ("decode_num",
+   ``decode_num p l =
+     case l of
+        (T :: T :: t) -> if p 0 then SOME (0, t) else NONE
+     || (T :: F :: t) ->
+        (case decode_num (K T) t of NONE -> NONE
+         || SOME (v, t') ->
+            if p (2 * v + 1) then SOME (2 * v + 1, t') else NONE)
+     || (F :: t) ->
+        (case decode_num (K T) t of NONE -> NONE
+         || SOME (v, t') ->
+            if p (2 * v + 2) then SOME (2 * v + 2, t') else NONE)
+     || _ -> NONE``,
+   (REPEAT CASE_TAC ++
+    RW_TAC std_ss [decode_num_def, enc2dec_none]) <<
+   [ONCE_REWRITE_TAC [encode_num_def]
+    ++ RW_TAC std_ss [APPEND],
+    ONCE_REWRITE_TAC [encode_num_def]
+    ++ RW_TAC std_ss [APPEND],
+    RW_TAC std_ss [enc2dec_some, wf_encode_num]
+    ++ ONCE_REWRITE_TAC [encode_num_def]
+    ++ RW_TAC std_ss [APPEND],
+    ONCE_REWRITE_TAC [encode_num_def]
+    ++ RW_TAC std_ss [APPEND]
+    ++ METIS_TAC [],
+    ONCE_REWRITE_TAC [encode_num_def]
+    ++ RW_TAC std_ss [APPEND]
+    ++ STRIP_TAC
+    ++ RW_TAC std_ss []
+    ++ Suff `encode_num = dec2enc (decode_num (K T))`
+    >> (STRIP_TAC
+        ++ Q.PAT_ASSUM `X = NONE` MP_TAC
+        ++ RW_TAC std_ss []
+        ++ MP_TAC (Q.SPEC `K T` wf_decode_num)
+        ++ Q.SPEC_TAC (`decode_num (K T)`, `d`)
+        ++ Q.SPEC_TAC (`(x - 1) DIV 2`, `x`)
+        ++ POP_ASSUM_LIST (K ALL_TAC)
+        ++ REPEAT STRIP_TAC
+        ++ MP_TAC
+           (Q.SPECL [`K T`, `d`, `x`, `t`]
+            (INST_TYPE [alpha |-> ``:num``] decode_dec2enc_append))
+        ++ RW_TAC std_ss [K_THM])
+    ++ RW_TAC std_ss [decode_num_def]
+    ++ MATCH_MP_TAC EQ_EXT
+    ++ RW_TAC std_ss [dec2enc_enc2dec, K_THM, wf_encode_num],
+    ASM_SIMP_TAC std_ss [enc2dec_some, wf_encode_num, APPEND]
+    ++ ONCE_REWRITE_TAC [encode_num_def]
+    ++ RW_TAC arith_ss [APPEND, GSYM ADD1, EVEN_ODD, ODD_DOUBLE]
+    ++ ONCE_REWRITE_TAC [MULT_COMM]
+    ++ RW_TAC std_ss [MULT_DIV]
+    ++ MP_TAC
+       (Q.SPECL [`K T`, `decode_num (K T)`]
+        (INST_TYPE [alpha |-> ``:num``] wf_decoder_def))
+    ++ ASM_SIMP_TAC std_ss [wf_decode_num]
+    ++ DISCH_THEN (MP_TAC o Q.SPEC `q`)
+    ++ RW_TAC std_ss [K_THM]
+    ++ RES_TAC
+    ++ RW_TAC std_ss [APPEND_11]
+    ++ POP_ASSUM (MP_TAC o Q.SPECL [`a`, `[]`])
+    ++ RW_TAC std_ss [APPEND_NIL, decode_num_def, enc2dec_some, wf_encode_num],
+    ONCE_REWRITE_TAC [encode_num_def]
+    ++ RW_TAC std_ss [APPEND]
+    ++ STRIP_TAC
+    ++ RW_TAC std_ss []
+    ++ Q.PAT_ASSUM `X = SOME Y` MP_TAC
+    ++ MP_TAC
+       (Q.SPECL [`K T`, `decode_num (K T)`]
+        (INST_TYPE [alpha |-> ``:num``] wf_decoder_def))
+    ++ ASM_SIMP_TAC std_ss [wf_decode_num]
+    ++ DISCH_THEN (MP_TAC o Q.SPEC `q`)
+    ++ RW_TAC std_ss [K_THM]
+    ++ RW_TAC std_ss []
+    ++ 
+    ++ POP_ASSUM (MP_TAC o Q.SPECL [`a`, `[]`])
+    ++ RW_TAC std_ss [APPEND_NIL, decode_num_def, enc2dec_some, wf_encode_num],
+
+
+
+    ++ Know `decode_num (K T) q = a`
+    >> PROVE_TAC [APPEND_NIL, dec2enc_some, wf_decode_num] ++
+    RW_TAC std_ss [APPEND_11] ++
+    Q.PAT_ASSUM `!x. P x` (K ALL_TAC) ++
+    MP_TAC
+    (Q.ISPECL [`EVERY (p : 'a -> bool)`, `decode_num (EVERY p) d`]
+     wf_decoder_def) ++
+    ASM_SIMP_TAC std_ss [] ++
+    DISCH_THEN (MP_TAC o Q.SPEC `q'`) ++
+    RW_TAC std_ss [] ++
+    RES_TAC ++
+    RW_TAC std_ss [] ++
+    Q.PAT_ASSUM `!x. P x` (K ALL_TAC) ++
+    Q.PAT_ASSUM `X = Y` MP_TAC ++
+    ASM_SIMP_TAC std_ss [decode_num_def, enc2dec_some],
+    Know `wf_decoder (EVERY p) (decode_num (EVERY p) d)` >>
+    PROVE_TAC [wf_decode_num] ++
+    STRIP_TAC ++
+    Know `wf_encoder p (dec2enc d)` >> PROVE_TAC [wf_dec2enc] ++
+    STRIP_TAC ++
+    Know `wf_encoder (EVERY p) (encode_num (dec2enc d))` >>
+    PROVE_TAC [wf_encode_num] ++
+    STRIP_TAC ++
+    ASM_SIMP_TAC std_ss [enc2dec_some, encode_num_def, APPEND, EVERY_DEF]]);
+*)
+
+(*---------------------------------------------------------------------------
      Trees
  ---------------------------------------------------------------------------*)
 
-val dec_tree_def = Define
-  `dec_tree p d = enc2dec p (encode_tree (dec2enc d))`;
+val decode_tree_def = Define
+  `decode_tree p d = enc2dec p (encode_tree (dec2enc d))`;
 
-val decode_tree_def = Define `decode_tree p d = decode (dec_tree p d)`;
-
-val wf_dec_tree = store_thm
-  ("wf_dec_tree",
+val wf_decode_tree = store_thm
+  ("wf_decode_tree",
    ``!p d.
        wf_decoder p d ==>
-       wf_decoder (lift_tree p) (dec_tree (lift_tree p) d)``,
-   RW_TAC std_ss [dec_tree_def] ++
+       wf_decoder (lift_tree p) (decode_tree (lift_tree p) d)``,
+   RW_TAC std_ss [decode_tree_def] ++
    PROVE_TAC [wf_dec2enc, wf_enc2dec, wf_encode_tree]);
 
-val dec_tree = store_thm
-  ("dec_tree",
+val decode_tree = store_thm
+  ("decode_tree",
    ``wf_decoder p d ==>
-     (dec_tree (lift_tree p) d l =
+     (decode_tree (lift_tree p) d l =
       case d l of NONE -> NONE
       || SOME (a, t) ->
-         (case dec_list (EVERY (lift_tree p))
-               (dec_tree (lift_tree p) d) t
+         (case decode_list (EVERY (lift_tree p))
+               (decode_tree (lift_tree p) d) t
           of NONE -> NONE
           || SOME (ts, t') -> SOME (Node a ts, t')))``,
    STRIP_TAC ++
-   Know `wf_decoder (lift_tree p) (dec_tree (lift_tree p) d)` >>
-   PROVE_TAC [wf_dec_tree] ++
+   Know `wf_decoder (lift_tree p) (decode_tree (lift_tree p) d)` >>
+   PROVE_TAC [wf_decode_tree] ++
    STRIP_TAC ++
    Know `wf_decoder (EVERY (lift_tree p))
-         (dec_list (EVERY (lift_tree p)) (dec_tree (lift_tree p) d))` >>
-   PROVE_TAC [wf_dec_list] ++
+         (decode_list (EVERY (lift_tree p)) (decode_tree (lift_tree p) d))` >>
+   PROVE_TAC [wf_decode_list] ++
    STRIP_TAC ++
    REPEAT CASE_TAC <<
-   [RW_TAC std_ss [dec_tree_def, enc2dec_none] ++
+   [RW_TAC std_ss [decode_tree_def, enc2dec_none] ++
     STRIP_TAC ++
     RW_TAC std_ss [] ++
     Q.PAT_ASSUM `X = Y` MP_TAC ++
@@ -406,7 +872,7 @@ val dec_tree = store_thm
     RW_TAC std_ss [lift_tree_def] ++
     MP_TAC (Q.SPECL [`p`, `d`, `a`] decode_dec2enc_append) ++
     RW_TAC std_ss [],
-    RW_TAC std_ss [dec_tree_def, enc2dec_none] ++
+    RW_TAC std_ss [decode_tree_def, enc2dec_none] ++
     STRIP_TAC ++
     RW_TAC std_ss [] ++
     Q.PAT_ASSUM `X = SOME Y` MP_TAC ++
@@ -426,16 +892,16 @@ val dec_tree = store_thm
     CONV_TAC (DEPTH_CONV ETA_CONV) ++
     STRIP_TAC ++
     MP_TAC (Q.SPECL [`lift_tree p`, `encode_tree (dec2enc d)`, `l`, `t`]
-            (INST_TYPE [alpha |-> ``:'a tree``] encode_then_dec_list)) ++
+            (INST_TYPE [alpha |-> ``:'a tree``] encode_then_decode_list)) ++
     MATCH_MP_TAC (PROVE [] ``(y ==> z) /\ x ==> (x ==> y) ==> z``) ++
-    CONJ_TAC >> RW_TAC std_ss [dec_tree_def] ++
+    CONJ_TAC >> RW_TAC std_ss [decode_tree_def] ++
     PROVE_TAC [wf_encode_tree, wf_dec2enc],
     MP_TAC
     (Q.SPECL [`lift_tree p`, `encode_tree (dec2enc d)`, `l`, `Node q q'`, `r'`]
      (INST_TYPE [alpha |-> ``:'a tree``] enc2dec_some)) ++
     MATCH_MP_TAC (PROVE [] ``x /\ (y ==> z) ==> (x ==> y) ==> z``) ++
     CONJ_TAC >> PROVE_TAC [wf_encode_tree, wf_dec2enc] ++
-    DISCH_THEN (fn th => SIMP_TAC std_ss [dec_tree_def, th]) ++
+    DISCH_THEN (fn th => SIMP_TAC std_ss [decode_tree_def, th]) ++
     SIMP_TAC std_ss [encode_tree_def, GSYM APPEND_ASSOC, lift_tree_def] ++
     CONV_TAC (DEPTH_CONV ETA_CONV) ++
     Suff
@@ -448,13 +914,13 @@ val dec_tree = store_thm
      PROVE_TAC [enc2dec_dec2enc] ++
      RW_TAC std_ss [enc2dec_some, wf_dec2enc],
      POP_ASSUM MP_TAC ++
-     SIMP_TAC std_ss [dec_list_def] ++
+     SIMP_TAC std_ss [decode_list_def] ++
      RW_TAC std_ss [enc2dec_some, wf_dec2enc, wf_encode_list, APPEND_11] ++
      Q.PAT_ASSUM `X = Y` (K ALL_TAC) ++
      Induct_on `q'` ++
      RW_TAC std_ss [EVERY_DEF, encode_list_def, APPEND_11] ++
      RW_TAC std_ss
-     [dec_tree_def, dec2enc_enc2dec, wf_dec2enc, wf_encode_tree]]]);
+     [decode_tree_def, dec2enc_enc2dec, wf_dec2enc, wf_encode_tree]]]);
 
 val _ = export_theory ();
 
